src/mapping/PStoRMWUtils.v
@@ -1,0 +1,100 @@
+Require Import NArith.
+Require Import PArith.
+Require Import ZArith.
+Require Import Lia.
+Require Import EquivDec.
+Require Import RelationClasses.
+
+From sflib Require Import sflib.
+From Paco Require Import paco.
+
+From PromisingLib Require Import Basic.
+From PromisingLib Require Import Axioms.
+From PromisingLib Require Import Language.
+From PromisingLib Require Import Event.
+From PromisingLib Require Import Loc.
+
+From PromisingIR Require Import Time.
+From PromisingIR Require Import View.
+From PromisingIR Require Import BoolMap.
+From PromisingIR Require Import Promises.
+From PromisingIR Require Import Reserves.
+From PromisingIR Require Import Cell.
+From PromisingIR Require Import Memory.
+From PromisingIR Require Import TView.
+From PromisingIR Require Import Global.
+From PromisingIR Require Import Local.
+From PromisingIR Require Import Thread.
+
+Require Import PromisingArch.lib.Basic.
+Require Import PromisingArch.lib.Order.
+Require Import PromisingArch.lib.Time.
+Require Import PromisingArch.lib.Lang.
+
+Require Import PromisingArch.promising.Promising.
+Require Import PromisingArch.mapping.RMWLang.
+Require Import PromisingArch.mapping.RMWPromising.
+Require Import PromisingArch.mapping.PSLang.
+
+Set Implicit Arguments.
+
+Module PSLoc := PromisingLib.Loc.Loc.
+Module PSTime := PromisingIR.Time.Time.
+Module PSView := PromisingIR.View.View.
+Module PSPromises := PromisingIR.Promises.Promises.
+Module PSLocal := PromisingIR.Local.Local.
+Module PSMemory := PromisingIR.Memory.Memory.
+
+
+Fixpoint ntt (n: nat): PSTime.t :=
+  match n with
+  | O => PSTime.bot
+  | S n => PSTime.incr (ntt n)
+  end.
+
+Lemma le_ntt
+  m n
+  (LE: m <= n):
+  PSTime.le (ntt m) (ntt n).
+Proof.
+  induction LE; try refl.
+  etrans; eauto. ss. econs.
+  apply PSTime.incr_spec.
+Qed.
+
+Lemma lt_ntt
+  m n
+  (LT: m < n):
+  PSTime.lt (ntt m) (ntt n).
+Proof.
+  eapply TimeFacts.lt_le_lt; try eapply le_ntt; eauto.
+  apply PSTime.incr_spec.
+Qed.
+
+Lemma ntt_le
+  m n
+  (LE: PSTime.le (ntt m) (ntt n)):
+  m <= n.
+Proof.
+  destruct (Nat.le_gt_cases m n); ss.
+  apply lt_ntt in H. timetac.
+Qed.
+
+Lemma ntt_lt
+  m n
+  (LT: PSTime.lt (ntt m) (ntt n)):
+  m < n.
+Proof.
+  destruct (Nat.le_gt_cases n m); ss.
+  apply le_ntt in H. timetac.
+Qed.
+
+Lemma ntt_inj
+  m n
+  (EQ: ntt m = ntt n):
+  m = n.
+Proof.
+  apply le_antisym.
+  - apply ntt_le. rewrite EQ. refl.
+  - apply ntt_le. rewrite EQ. refl.
+Qed.
